\input ../talk-header.tex
\title
{Machine Learning}
\subtitle{Logistic Regression}

\begin{document}

\maketitle

\begin{frame}
  \vphrase{Review of Linear Regression}
\end{frame}

\begin{frame}{Linear models}

  \only<1>{
    \textbf{Problem:}  $\{(x_i, y_i)\}$.

    Given $x$, predict $\hat y$.
  }

  \only<2>{ $x$: \textbf{explanatory} or \textbf{predictor} variable.  Or the \textbf{signal}.

    $y$: \textbf{response} variable.

    \vspace{1cm}
    \purple{For some reason, we believe a linear model is a good idea.}
  }
\end{frame}

\begin{frame}{Residuals}

  Residuals (model error):
  \begin{itemize}
  \item What's left over
  \item What the model doesn't explain
  \end{itemize}


  \only<1>{
    \vspace{1cm}
    \begin{displaymath}
      \text{data} = \text{fit} + \text{residual}      
    \end{displaymath}
  }
  \only<2>{
    \vspace{1cm}
    \begin{displaymath}
      y_i = \hat y_i + e_i
    \end{displaymath}
  }
  \only<3>{
    \vspace{1cm}
    \begin{displaymath}
      e_i = y_i - \hat y_i
    \end{displaymath}
  }
  \only<4>{
    Goal: small residuals.

    \vspace{1cm}
    \begin{displaymath}
      \sum e_i^2
    \end{displaymath}
  }
\end{frame}

\begin{frame}{Hypothesis (Model)}

  \only<1>{
    \begin{mphrase}
      y = a + bx
    \end{mphrase}
  }
  \only<2>{
    \begin{mphrase}
      h_\theta(x) = \theta_0 + \theta_1 x
    \end{mphrase}
  }
\end{frame}

\begin{frame}{Cost Function}
  Also called the ``loss function''.

  \only<1>{
    \begin{mphrase}
      J(\theta_0, \theta_1) = \frac{1}{2m} \sum_{i=1}^m (e_i)^2
    \end{mphrase}
  }
  \only<2>{
    \begin{mphrase}
      J(\theta_0, \theta_1) = \frac{1}{2m} \sum_{i=1}^m (\hat{y}_i - y_i)^2
    \end{mphrase}
  }
  \only<3>{
    \begin{mphrase}
      J(\theta_0, \theta_1) = \frac{1}{2m} \sum_{i=1}^m (h_\theta(x_i) - y_i)^2
    \end{mphrase}
  }
\end{frame}


\begin{frame}
  \cimgh{../J1-B/parameter-space.png}
\end{frame}



\begin{frame}{Gradient Descent}

  \only<1>{
    \begin{mphrase}
      \begin{dcases}
        \theta_0 & \leftarrow\, \theta_0 - \alpha
        \frac{\partial}{\partial\theta_0}\, J(\theta_0, \theta_1)
        \\[3mm]
        % 
        \theta_1 & \leftarrow\, \theta_1 - \alpha
        \frac{\partial}{\partial\theta_1}\, J(\theta_0, \theta_1)
      \end{dcases}
    \end{mphrase}
  }
  \only<2>{
    \begin{mphrase}
      \begin{dcases}
        \theta_0 & \leftarrow\, \theta_0 - \alpha
        \frac{\partial}{\partial\theta_0}\,
        \left(\frac{1}{2m} \sum_{i=1}^m (h_\theta(x_i) - y_i)^2\right)
        \\[3mm]
        % 
        \theta_1 & \leftarrow\, \theta_1 - \alpha
        \frac{\partial}{\partial\theta_1}\,
        \left(\frac{1}{2m} \sum_{i=1}^m (h_\theta(x_i) - y_i)^2\right)
      \end{dcases}
    \end{mphrase}
  }
  \only<3>{
    \begin{mphrase}
      \begin{dcases}
        \theta_0 & \leftarrow\, \theta_0 - \alpha
        \frac{\partial}{\partial\theta_0}\,
        \left(\frac{1}{2m} \sum_{i=1}^m (\theta_0 + \theta_1 x_i - y_i)^2\right)
        \\[3mm]
        % 
        \theta_1 & \leftarrow\, \theta_1 - \alpha
        \frac{\partial}{\partial\theta_1}\,
        \left(\frac{1}{2m} \sum_{i=1}^m (\theta_0 + \theta_1 x_i - y_i)^2\right)
      \end{dcases}
    \end{mphrase}
  }
  \only<4>{
    \begin{mphrase}
      \begin{dcases}
        \theta_0 & \leftarrow \, \theta_0 - 
        \frac{\alpha}{m} \sum_{i=1}^m ( \theta_0 + \theta_1 x_i - y_i ) \, 1
        \\[3mm]
        % 
        \theta_1 & \leftarrow \, \theta_1 -
        \frac{\alpha}{m} \sum_{i=1}^m (\theta_0 + \theta_1 x_i - y_i) - y_i) \, x_i
      \end{dcases}
    \end{mphrase}
  }
  \only<5>{
    \begin{mphrase}
      \begin{dcases}
        \theta_0 & \leftarrow \, \theta_0 - 
        \frac{\alpha}{m} \sum_{i=1}^m ( h_\theta(x_i) - y_i )
        \\[3mm]
        % 
        \theta_1 & \leftarrow \, \theta_1 -
        \frac{\alpha}{m} \sum_{i=1}^m (h_\theta(x_i) - y_i) \, x_i
      \end{dcases}
    \end{mphrase}
  }
\end{frame}

\begin{frame}
  \vphrase{Logistic regression}
\end{frame}

\begin{frame}
  \frametitle{Linear regression}
  \begin{bphrase}
    \begin{itemize}
    \item Inputs are continuous or discrete
    \item Continuous output
    \item Normal residues
    \item Predict $\hat{y}$ for $x$ given $\{(x_i, y_i)\}$
    \end{itemize}
  \end{bphrase}
\end{frame}

\begin{frame}
  \frametitle{Logistic regression}
  \begin{bphrase}
    \begin{itemize}
    \item Inputs are continuous or discrete
    \item Binary output
    \item Classification
    \end{itemize}
  \end{bphrase}
\end{frame}

\begin{frame}
  \frametitle{Logistic regression}
  \begin{itemize}
  \item Have: continuous and discrete inputs
  \item Want: class (0 or 1)
  \end{itemize}
\end{frame}

\begin{frame}{Logistic regression: motivation}
  % This slide left blank for drawing.
\end{frame}

\begin{frame}{Probabilistic inspiration}
  \purple{The probabilities are motivations: this doesn't really behave like a probability.}
  
  \only<1>{
    \sphrase{{$h_\theta(x) = .75$} $\iff$ {event has 75\% of being true}}
  }
  \only<2>{
    \sphrase{$h_\theta(x) = \Pr(y=1\mid x; \theta)$ = 0.75}
  }
  \only<3>{
    \sphrase{So this must be true:}
    
    \sphrase{$\Pr(y=0\mid x; \theta) + \Pr(y=1\mid x; \theta)$ = 1}
  }
  \only<4>{
    \sphrase{Set $y=1 \iff h_\theta(x) = \Pr(y=1\mid x; \theta) > \frac{1}{2}$}
  }
  \only<5-6>{
    Let
    \begin{align*}
      Pr(y=0\mid x; \theta) & = h_\theta(x) \\
      Pr(y=1\mid x; \theta) & = 1 - h_\theta(x) \\
    \end{align*}
    \only<6>{
      Then
      \begin{displaymath}
        Pr(y=0\mid x; \theta) + \Pr(y=1\mid x; \theta) = 1
      \end{displaymath}
    }
  }
  \only<7>{
    Math review:
    \begin{itemize}
    \item $z=(\theta^T x)$
    \item $\theta^T x \ge 0 \iff h_\theta \ge 0.5$
    \item $\theta^T x \ge 0 \iff $ predict $y=1$
    \end{itemize}

    }
\end{frame}

\begin{frame}[t]{Logistic (sigmoid) function}
  \vspace{2cm}
  \begin{mphrase}
    \sigma(z) = \frac{e^z}{e^z  +1} = \frac{1}{1+e^{-z}}
  \end{mphrase}

  \only<2>{
    \vspace{8mm}
    Exercise: plot this
  }
  \only<3>{
    Let
    \begin{displaymath}
      z = h_\theta(x) = \theta_0 + \theta_1 x
    \end{displaymath}

  }
  \only<4>{
    Then
    \begin{displaymath}
      \sigma(z) = \frac{1}{1 + e^{-(\theta_0 + \theta_1 x)}}
    \end{displaymath}

    }
\end{frame}

\begin{frame}[t]{Cost function in logistic regression}
  \vspace{1cm}
  \purple{In linear regression, we had}
  
  \begin{displaymath}
    \only<1>{J(\theta) = \frac{1}{2m} \sum_{i=1}^m (e_i)^2}
    \only<2>{J(\theta) = \frac{1}{2m} \sum_{i=1}^m (\hat{y}_i - y_i)^2}
    \only<3>{J(\theta) = \frac{1}{2m} \sum_{i=1}^m (h_\theta(x_i) - y_i)^2}
    \only<4>{J(\theta) = \frac{1}{2m} \sum_{i=1}^m (h_\theta(x) - y)^2}
  \end{displaymath}
\end{frame}

\begin{frame}[t]{Cost function in logistic regression}
  \vspace{1cm}
  \purple{To do gradient descent, we need the derivative of the cost function.}
  \only<1-3>{
    \begin{align*}
      g(z) & = \frac{1}{1-e^{-z}}
    \end{align*}
  }
  \begin{align*}
    \only<2->{
    \frac{dg}{dz}
    }
    \only<2-4>{
    & = \frac{-1}{\left( 1 - e^{-z}\right)^2} \cdot \left(e^{-z}\right) \\[2mm]
    }
    \only<3-5>{
    & = \frac{e^{-z}}{\left( 1 - e^{-z}\right)^2} \\[2mm]
    }
    \only<4-6>{
    & = \frac{e^{-z}}{\left( 1 - e^{-z}\right)\left( 1 - e^{-z}\right)} \\[2mm]
    }
    \only<5-7>{
    & = \left(\frac{1}{1 - e^{-z}}\right) \left(\frac{e^{-z}}{1 - e^{-z}}\right) \\[2mm]
    }
    \only<6-8>{
    & = \left(\frac{1}{1 - e^{-z}}\right) \left(\frac{1 - \left(1 - e^{-z}\right)}{1 - e^{-z}}\right) \\[2mm]
    }
    \only<7-9>{
    & = \left(\frac{1}{1 - e^{-z}}\right) \left( 1 - \frac{1}{1 - e^{-z}}\right) \\[2mm]
    }
    \only<8-11>{
    & = g(z) (1-g(z))
      }
  \end{align*}
  
  \only<11>{
    \vspace{1cm}
    \purple{And for today we'll stop there.}
  }
\end{frame}

\begin{frame}
  \vspace{1cm}

  \only<1>{\phrase{null hypothesis}}
  \only<2>{\phrase{true positive, true negative}
    \vspace{1cm}
    \phrase{false positive, false negative}}
  \only<3>{\phrase{type I error}
  \centerline{(incorrect rejection of null hypothesis)}
    \vspace{1cm}
    \phrase{type II error}
    \centerline{(failure to reject null hypothesis)}}
  \only<4>{\phrase{sensitivity}\centerline{100\% sensitivity = no false negatives}}
  \only<5>{\phrase{specificity}\centerline{100\% specificity = no false positives}}
\end{frame}

\begin{frame}{Precision}
  \vspace{1cm}

  \begin{mphrase}
    P = \frac{TP}{TP + FP}
  \end{mphrase}
\end{frame}

\begin{frame}{Recall}
  \vspace{1cm}

  \begin{mphrase}
    R = \frac{TP}{TP + FN}
  \end{mphrase}
\end{frame}

\begin{frame}{F1 score}
  \vspace{1cm}

  \begin{mphrase}
    F1 = \frac{\text{precision}\cdot\text{recall}}{\text{precision} + \text{recall}}
  \end{mphrase}
\end{frame}

\begin{frame}
  \frametitle{Non-linear decision boundaries}
  \only<1> {
    \cimggg{non-linear-boundary.png}
    \sphrase{$h_\theta(x)) = g(\theta_0 + \theta_1 x_1 + \theta_2 x_2 + \theta_3 x_1^2 + \theta_4 x_2^2$}

    \vfill
    \prevwork{Andrew Ng}
  }
  \only<2> {
    \sphrase{OvA = OvR}
    \vspace{1cm}
    \sphrase{OvO}
  }
  \only<3> {
    \sphrase{One vs All = One vs Rest}
    \vspace{1cm}
    \sphrase{One vs One}
  }
\end{frame}

\begin{frame}{Scikit Learn}
  \lstinputlisting{sk_linreg.py}
\end{frame}

\begin{frame}{Scikit Learn}
  \lstinputlisting{sk_logreg.py}
\end{frame}

\end{document}
